Added extended_monoid_inv_def

examples/algebra/monoid/monoidOrderScript.sml
@@ -1068,18 +1068,35 @@ val monoid_inv_from_invertibles = store_thm(
   ``!g:'a monoid. Monoid g ==> !x. x IN G* ==> ?y. y IN G /\ (x * y = #e) /\ (y * x = #e)``,
   rw[monoid_invertibles_def]);
 
-(* Convert this into the form: !g x. ?y. ..... for SKOLEM_THM *)
-val lemma = prove(``!(g:'a monoid) x. ?y. Monoid g /\ x IN G* ==> y IN G /\ (x * y = #e) /\ (y * x = #e)``,
+(* Convert this into the form: !g x. ?y. ..... for SKOLEM_THM
+val lemma = prove(
+  ``!(g:'a monoid) x. ?y. Monoid g /\ x IN G* ==> y IN G /\ (x * y = #e) /\ (y * x = #e)``,
   metis_tac[monoid_inv_from_invertibles]);
+ *)
+
+(* Convert this into the form: !g x. ?y. ..... for SKOLEM_THM
+
+   NOTE: added ‘(Monoid g /\ x NOTIN G* ==> y = ARB)’ to make it a total function.
+ *)
+val lemma = prove(
+   “!(g:'a monoid) x. ?y. (Monoid g /\ x IN G* ==> y IN G /\ (x * y = #e) /\ (y * x = #e)) /\
+                          (Monoid g /\ x NOTIN G* ==> y = ARB)”,
+    rpt GEN_TAC
+ >> MP_TAC (Q.SPEC ‘g’ monoid_inv_from_invertibles)
+ >> Cases_on ‘Monoid g’ >> rw []
+ >> Cases_on ‘x IN G*’ >> rw []);
 
 (* Use Skolemization to generate the monoid_inv_from_invertibles function *)
-val monoid_inv_def = new_specification(
-  "monoid_inv_def",
+val extended_monoid_inv_def = new_specification(
+   "extended_monoid_inv_def",
   ["monoid_inv"], (* name of function *)
   SIMP_RULE (srw_ss()) [SKOLEM_THM] lemma);
-(* > val monoid_inv_def = |- !g x. Monoid g /\ x IN G* ==>
-         monoid_inv g x IN G /\ (x * monoid_inv g x = #e) /\ (monoid_inv g x * x = #e) : thm *)
 
+(* |- !g x. Monoid g /\ x IN G* ==>
+            monoid_inv g x IN G /\ (x * monoid_inv g x = #e) /\
+                                   (monoid_inv g x * x = #e)
+ *)
+Theorem monoid_inv_def = cj 1 full_monoid_inv_def
 (*
 - type_of ``monoid_inv g``;
 > val it = ``:'a -> 'a`` : hol_type
